\documentclass{article}
\usepackage[left=3cm,right=3cm,top=3cm,bottom=3cm]{geometry}
\usepackage{amsmath,amssymb,amsthm,pgfplots,tikz}
\usepackage[inline]{enumitem}
\usepackage{color}
\setlength{\parindent}{0mm} %So that we do not indent on new paragraphs
\newcommand{\TODO}[1]{\textcolor{red}{TODO: #1}}

\begin{document}
\title{Graduate Algebra II: Homework 3}
\author{Li Ling Ko\\ lko@nd.edu}
\date{\today}
\maketitle

\it \textbf{Q1:} Let $A$ and $B$ be abelian groups, and $m,n$ positive
  integers.
  \begin{enumerate}[label={(\alph*)}]
    \item Show that $A\otimes_\mathbb{Z}\mathbb{Z}_m \cong A/mA$.
      \begin{proof}
        Consider the map $\varphi:A\times\mathbb{Z}_m
        \rightarrow A/mA$ defined by
        $(a,\bar{z})\mapsto\overline{z\cdot a}$. We first show this map
        is well-defined and $\mathbb{Z}$-bilinear. To show that the map is
        well-defined, we have
        \begin{align*}
          \varphi((a,\overline{z+m})) &=\overline{(z+m)\cdot a}\\
          &=\overline{z\cdot a+m\cdot a}\\
          &=\overline{z\cdot a}\\
          &=\varphi((a,\overline{z})).\\
        \end{align*}

        To show $\mathbb{Z}$-bilinearlity, we have
        \begin{align*}
          \varphi(((a_1+a_2),\overline{z})) &=\overline{z\cdot
            (a_1+a_2)}\\
          &=\overline{z\cdot a_1 +z\cdot a_2}\\
          &=\overline{z\cdot a_1} +\overline{z\cdot a_2}\\
          &=\varphi((a_1,\overline{z}))
            +\varphi((a_2,\overline{z})),\\
        \end{align*}

        and
        \begin{align*}
          \varphi((a,(\overline{z_1}+\overline{z_2})))
            &=\varphi((a,(\overline{z_1+z_2})))\\
          &=\overline{(z_1+z_2)\cdot a}\\
          &=\overline{z_1\cdot a +z_2\cdot a}\\
          &=\overline{z_1\cdot a} +\overline{z_2\cdot a}\\
          &=\varphi((a,\overline{z_1}))
            +\varphi((a,\overline{z_2})),\\
        \end{align*}

        and
        \begin{align*}
          \varphi((n\cdot a,\overline{z})))
          &=\overline{z\cdot (n\cdot a)}\\
          &=\overline{(nz)\cdot a}\\
          &=\overline{(n\cdot\overline{z})\cdot a}\\
          &=\varphi((a, (n\cdot \overline{z}))),\\
        \end{align*}

        and
        \begin{align*}
          \varphi((a,n\cdot\overline{z}))
          &=\varphi((a,\overline{nz}))\\
          &=\overline{(nz)\cdot a}\\
          &=\overline{(n\cdot\overline{z})\cdot a}\\
          &=\varphi((a, (n\cdot \overline{z}))).\\
        \end{align*}

        Thus from Corollary 12, $\varphi$ induces a $\mathbb{Z}$-module
        homomorphism $\Phi:A\otimes_\mathbb{Z}\mathbb{Z}_m \rightarrow
        A/mA$ defined by $\Phi(a\otimes\bar{z})=\overline{z\cdot a}$. Now
        $\Phi$ is clearly surjective since every $\overline{a}\in
        A/mA$ has a pre-image $a\otimes\bar{1}$. It remains to show that
        $\Phi$ is injective. Now by definition, every element $x$ of
        $A\otimes_\mathbb{Z}\mathbb{Z}_m$ can be written
        \[x=\sum_{i=1}^n a_i\otimes\overline{z_i}\]
        for some $a_i\in A$, $\overline{z_i}\in\mathbb{Z}_m$. Thus
        \begin{align*}
          \;&x\in\ker(\Phi)\\
          \Leftrightarrow\;&\sum_{i=1}^n a_i\otimes\overline{z_i}
            \in\ker(\Phi)\\
          \Leftrightarrow\;&\sum_{i=1}^n \overline{z_i\cdot
            a_i}=\overline{0}\in A/mA\\
          \Leftrightarrow\;&\overline{\sum_{i=1}^n z_i\cdot
            a_i}=\overline{0}\in A/mA\\
          \Leftrightarrow\;&\sum_{i=1}^n z_i\cdot a_i\in mA\\
          \Leftrightarrow\;&\sum_{i=1}^n z_i\cdot a_i =m\cdot b\in A\;
            \text{for some}\; b\in A\\
          \Rightarrow\;&\left(\sum_{i=1}^n z_i\cdot a_i\right)
            \otimes\bar{1}=(m\cdot b)\otimes\bar{1}\; \text{for some}\;
            b\in A.\\
          \Rightarrow\;&\sum_{i=1}^n (z_i\cdot a_i)\otimes\bar{1} =(m\cdot
            b)\otimes\bar{1}\; \text{for some}\; b\in A.\\
        \end{align*}

        Now by $\mathbb{Z}$-bilinear property of tensors, given arbitrary
        $a\in A$ and $z\in\mathbb{Z}_m$,
        \begin{align*}
          &\;(z\cdot a)\otimes\bar{1}\\
          =&\;a\otimes(z\cdot\bar{1})\\
          =&\;a\otimes\bar{z},\\
        \end{align*}
        thus we can simplify the above conditions to get
        \[\sum_{i=1}^n a_i\otimes\overline{z_i} =b\otimes\overline{m}=0,\]
        which implies $x=0$. Thus $\ker(\Phi)=0$.
      \end{proof}

    \item Show that $\mathbb{Z}_m\otimes_\mathbb{Z}\mathbb{Z}_n
      \cong\mathbb{Z}_c$, where $c=(m,n)$.
      \begin{proof}
        By replacing $m$ with $n$ in part (a) of this question letting
        $A=\mathbb{Z}_m$, it suffices to show that
        $\mathbb{Z}_m/n\mathbb{Z}_m\cong \mathbb{Z}_c$ as
        $\mathbb{Z}$-modules. First, observe that
        $n\mathbb{Z}_m=c\mathbb{Z}$: $c$ is the smallest positive integer
        such that there exists $x_0,y_0\in\mathbb{Z}$ with $c=x_0m+y_0n$.
        Thus in $\mathbb{Z}_m$,
        $\overline{c}=\overline{x_0m+y_0n}=\overline{y_0n}=n\overline{y_0}
        \in n\mathbb{Z}_m$. Also, since all elements in $n\mathbb{Z}_m$
        should be of the form $xm+yn$ for some $x,y\in\mathbb{Z}$, and $c$
        is the smallest positive integer of such form, and $n\mathbb{Z}_m$
        is closed under multiplication modulo $m$, $n\mathbb{Z}_m$ must
        equal
        \[n\mathbb{Z}_m =\{\overline{0}, \overline{c},
        \overline{2c}, \ldots, \overline{m-c}\}=c\mathbb{Z}_m.\]

        Therefore
        \[\mathbb{Z}_m/n\mathbb{Z}_m =\mathbb{Z}_m/c\mathbb{Z}_m
        \cong\mathbb{Z}_c.\]
      \end{proof}

    \item If $A$ is a torsion group (i.e. a torsion $\mathbb{Z}$-module),
      then $A\otimes_\mathbb{Z}\mathbb{Q}=0$.

      \begin{proof}
        Every element in $x\in A\otimes_\mathbb{Z}\mathbb{Q}$ can be
        written as a finite sum
        \[x=\sum_{i=1}^k a_i\otimes q_i\]
        for some $a_i\in A$, $q_i\in \mathbb{Q}$ by definition of torsion
        products. Since $A$ is torsion, for each $i=\{1,\ldots,k\}$,
        there exists $n_i$ such that $n_i\cdot a_i=0$. Let $n=n_1\cdots
        n_k$. Then $n\cdot a_i=0$ for all $i=\{1,\ldots,k\}$. So
        \begin{align*}
          &\;a_i\otimes q_i\\
          =&\;a_i\otimes(n\cdot(q_i/n))\\
          =&\;(n\cdot a_i)\otimes(q_i/n)\\
          =&\;0\otimes(q_i/n)\\
          =&\;(0\cdot0)\otimes(q_i/n)\\
          =&\;0\otimes(0\cdot q_i/n)\\
          =&\;0\otimes0\\
          =&\;0,\\
        \end{align*}
        thus
        \[x=\sum_{i=1}^k a_i\otimes q_i =\sum_{i=1}^k 0=0.\]
      \end{proof}
  \end{enumerate}

\it \textbf{Q2:} What is the difference between the homomorphism $f\otimes
  g$ as defined in class, and the element $f\otimes g\in\text{Hom}_R(A,A')
  \otimes_\mathbb{Z}\text{Hom}_R(B,B')$?
  \begin{proof}
  \end{proof}

\it \textbf{Q3:}
  \begin{enumerate}[label={(\alph*)}]
    \item From Exercise 1, determine what
      $\mathbb{Z}_2\otimes_\mathbb{Z}\mathbb{Z}_2$ is as an abelian group,
      and what is $\mathbb{Z}_2\otimes_\mathbb{Z}\mathbb{Z}_4$ as an
      abelian group.

      \begin{proof}
        From Question 1b, $\mathbb{Z}_2\otimes_\mathbb{Z}\mathbb{Z}_2
        \cong\mathbb{Z}_2$ as a $\mathbb{Z}$-module, thus it is isomorphic
        to $\mathbb{Z}_2$ as an abelian group. Similarly,
        $\mathbb{Z}_2\otimes_\mathbb{Z}\mathbb{Z}_4$ is isomorphic to
        $\mathbb{Z}_2$ as an abelian group.
      \end{proof}

    \item Let $\phi:\mathbb{Z}_2\rightarrow\mathbb{Z}_4$ be the usual
      injection of abelian groups. Show that $1\otimes\phi:
      \mathbb{Z}_2\otimes_\mathbb{Z}\mathbb{Z}_2
      \rightarrow\mathbb{Z}_2\otimes_\mathbb{Z}\mathbb{Z}_4$, is the zero
      map, even though $\mathbb{Z}_2\otimes_\mathbb{Z}\mathbb{Z}_2$ and
      $\mathbb{Z}_2\otimes_\mathbb{Z}\mathbb{Z}_4$ are nontrivial.

      \begin{proof}
        Given arbitrary $a,b\in\mathbb{Z}_2$,
        \begin{align*}
          &\;(1\otimes\phi)(\overline{a}\otimes \overline{b})\\
          =&\;\overline{a}\otimes \overline{2b}
            \in\mathbb{Z}_2\otimes_\mathbb{Z}\mathbb{Z}_4\\
          =&\;\overline{2a}\otimes \overline{b}\\
          =&\;\overline{0}\otimes \overline{b} &(\because\; 2|2a)\\
          =&\;\overline{0}\otimes \overline{0}\\
          =&\;0\in\mathbb{Z}_2\otimes_\mathbb{Z}\mathbb{Z}_4.\\
        \end{align*}

        So since elements of $\mathbb{Z}_2\otimes_\mathbb{Z}\mathbb{Z}_2$
        are finite sums of elements of the form $a\otimes b$ with
        $a,b\in\mathbb{Z}_2$ and homomorphisms preserve addition, the image
        of any element in $\mathbb{Z}_2\otimes_\mathbb{Z}\mathbb{Z}_2$ will
        be a finite sum of $0$'s, which will remain 0.
      \end{proof}
  \end{enumerate}

\textbf{Let $R$ be a ring with 1.} \\

\it \textbf{Section 10.4 Q3:} Show that
  $\mathbb{C}\otimes_\mathbb{R}\mathbb{C}$ and
  $\mathbb{C}\otimes_\mathbb{C}\mathbb{C}$ are both left
  $\mathbb{R}$-modules but are not isomorphic as $\mathbb{R}$-modules.

  \begin{proof}
    $\mathbb{C}\otimes_\mathbb{R}\mathbb{C}$ is a left $\mathbb{R}$-module
    because $\mathbb{C}$ is trivally a $\mathbb{R}$-module. Similarly,
    $\mathbb{C}\otimes_\mathbb{C}\mathbb{C}$ is a left $\mathbb{C}$-module
    because $\mathbb{C}$ is trivially a $\mathbb{C}$-module. Then since
    $\mathbb{R}$ is a subring of $\mathbb{C}$ with the same unity,
    $\mathbb{C}\otimes_\mathbb{C}\mathbb{C}$ will also be a left
    $\mathbb{R}$-module. \\

    We first show that $\mathbb{C}\otimes_\mathbb{R}\mathbb{C}$ is
    isomorphic to $\mathbb{R}^4$ as $\mathbb{R}$-modules. Consider the map
    $\varphi:\mathbb{C}\times\mathbb{C}\rightarrow\mathbb{R}^4$ defined by
    $\varphi((a_0+b_0i,a_1+b_1i)) =(a_0a_1,a_0b_1,a_1b_0,b_0b_1)$, where
    $a_0,b_0,a_1,b_1\in\mathbb{R}$. It is routine to show that $\varphi$ is
    a $\mathbb{R}$-bilinear map: Given
    $r,a_0,b_0,a_1,b_1,c_0,d_0,c_1,d_1\in\mathbb{R}$,
    \begin{align*}
      \;&\varphi((ra_0+rb_0i,a_1+b_1i))\\
      =\;&(ra_0a_1,ra_0b_1,ra_1b_0,rb_0b_1)\\
      =\;&r\cdot(a_0a_1,a_0b_1,a_1b_0,b_0b_1)\\
      =\;&\varphi((a_0+b_0i,ra_1+rb_1i)),\\
      =\;&r\cdot(a_0a_1,a_0b_1,a_1b_0,b_0b_1)\\
      =\;&r\cdot\varphi((a_0+b_0i,a_1+b_1i)),\\
    \end{align*}

    and,
    \begin{align*}
      \;&\varphi((a_0+b_0i+c_0+d_0i, a_1+b_1i))\\
      =\;&(a_0a_1+c_0a_1, a_0b_1+c_0b_1, a_1b_0+a_1d_0, b_0b_1+d_0b_1)\\
      =\;&(a_0a_1,a_0b_1,a_1b_0,b_0b_1) +(c_0a_1,c_0b_1,a_1d_0,d_0b_1)\\
      =\;&\varphi((a_0+b_0i, a_1+b_1i)) +\varphi((c_0+d_0i, a_1+b_1i)).\\
    \end{align*}
    Similarly, we can show that
    \[\varphi((a_0+b_0i, a_1+b_1i+c_1+d_1i))
    =\varphi((a_0+b_0i, a_1+b_1i)) +\varphi((a_0+b_0i, c_1+c_1i)).\]

    Thus from Corollary 12, $\varphi$ induces an $\mathbb{R}$-module
    homomorphism $\Phi:\mathbb{C}\otimes_\mathbb{R}\mathbb{C}\rightarrow
    \mathbb{R}^4$ defined by
    $\Phi((a_0+b_0i)\otimes(a_1+b_1i))=(a_0,b_0,a_1,b_1)$. This map is
    trivially surjective, since arbitrary
    $(r_0,r_1,r_2,r_3)\in\mathbb{R}^4$ as pre-image
    $(r_0+r_1i)\otimes(r_2+r_3i)$. Thus the dimension of
    $\mathbb{C}\otimes_\mathbb{R}\mathbb{C}$ as an $\mathbb{R}$-module must
    be at least the dimension of $\mathbb{R}^4$, which is 4. \\

    Next, observe that $\mathbb{C}\otimes_\mathbb{C}\mathbb{C}$ can be
    spanned as an $\mathbb{R}$-module by two elements
    $\{1\otimes1,1\otimes i\}$, because given $a,b,c,d\in\mathbb{R}$, we can
    write
    \begin{align*}
      &\;(a+bi)\otimes(c+di)\\
      =&\;a\otimes c+a\otimes di +bi\otimes c +bi\otimes di\\
      =&\;ac\cdot(1\otimes1) +ad\cdot(1\otimes i) +bc\cdot(i\otimes1)
        +bd\cdot(i\otimes i)\\
      =&\;ac\cdot(1\otimes1) +ad\cdot(1\otimes i) +bc\cdot(1\otimes i)
        -bd\cdot(1\otimes1)\\
      =&\;(ac-bd)\cdot(1\otimes1) +(ad+bc)\cdot(1\otimes i),\\
    \end{align*}
    where the second last equality follows because $1\otimes i=i\otimes1$
    and $i\otimes i=-1\otimes1$ as the tensor is defined with respect to
    $\mathbb{C}$. \\

    Thus $\mathbb{C}\otimes_\mathbb{R}\mathbb{C}$ has $\mathbb{R}$-module
    dimension no greater than 2, while
    $\mathbb{C}\otimes_\mathbb{C}\mathbb{C}$ has $\mathbb{R}$-module
    dimension at least 4, so they cannot be isomorphic as
    $\mathbb{R}$-modules.
  \end{proof}

\it \textbf{Section 10.4 Q5:} Let $A$ be a finite abelian group of order
  $n$ and let $p^k$ be the largest power of the prime $p$ dividing $n$.
  Prove that $\mathbb{Z}_{p^k}\otimes_\mathbb{Z}A$ is isomorphic to
  the Sylow $p$-subgroup of $A$.

  \begin{proof}
    Let the elementary divisor decomposition of $A$ be
    \[A\cong P\oplus_{i=1}^m\mathbb{Z}_{q_i^{\alpha_i}},\]
    where the $q_i$'s are distinct primes from $p$, and
    \[P=\mathbb{Z}_{p^{\alpha_1}}
    \oplus\ldots\oplus\mathbb{Z}_{p^{\alpha_n}}\]
    is the Sylow $p$-subgroup of $A$. Note that the decomposition is
    expressed as direct sum of $\mathbb{Z}$-modules. Then
    \begin{align*}
      &\;\mathbb{Z}_{p^k}\otimes_{\mathbb{Z}}A\\
      =&\;\mathbb{Z}_{p^k}\otimes_{\mathbb{Z}}
        (P\oplus_{i=1}^m \mathbb{Z}_{q_i^{\alpha_i}})\\
      =&\;(\mathbb{Z}_{p^k}\otimes_{\mathbb{Z}}P)
        \oplus(\mathbb{Z}_{p^k}
        \otimes_{\mathbb{Z}}\mathbb{Z}_{q_1^{\alpha_1}}) \oplus\ldots
        \oplus(\mathbb{Z}_{p^k}
        \otimes_{\mathbb{Z}}\mathbb{Z}_{q_m^{\alpha_m}}).
        &(\text{distributive property of tensors})\\
    \end{align*}

    Now for each $i\in\{1,\ldots,m\}$, since $p$ and $q_i$ are distinct
    primes, we have from Question 1b that
    \[\mathbb{Z}_{p^k} \otimes_{\mathbb{Z}}\mathbb{Z}_{q_m^{\alpha_m}}
    \cong\mathbb{Z}_1.\]

    Therefore
    \begin{align*}
      &\;\mathbb{Z}_{p^k}\otimes_{\mathbb{Z}}A\\
      =&\;(\mathbb{Z}_{p^k}\otimes_{\mathbb{Z}}P)
        \oplus(\mathbb{Z}_{p^k}
        \otimes_{\mathbb{Z}}\mathbb{Z}_{q_1^{\alpha_1}}) \oplus\ldots
        \oplus(\mathbb{Z}_{p^k}
        \otimes_{\mathbb{Z}}\mathbb{Z}_{q_m^{\alpha_m}})\\
      =&\;(\mathbb{Z}_{p^k}\otimes_{\mathbb{Z}}P) \oplus\mathbb{Z}_1
        \oplus\ldots \oplus\mathbb{Z}_1\\
      =&\;\mathbb{Z}_{p^k}\otimes_{\mathbb{Z}}P.\\
    \end{align*}
  \end{proof}

\it \textbf{Section 10.4 Q7:} If $R$ is any integral domain with quotient
  field $Q$ and $N$ is a left $R$-module, prove that every element of the
  tensor product $Q\otimes_R N$ can be written as a simple tensor of the
  form $(1/d)\otimes n$ for some nonzero $d\in R$ and some $n\in N$.

  \begin{proof}
    Let $q\in Q$ and $n'\in N$ be arbitrary. Then $q=c/d$ for some $c,d\in
    R$ and $d\neq0$, thus
    \begin{align*}
      &\;q\otimes n'\\
      =&\;(c/d)\otimes n'\\
      =&\;c\cdot((1/d)\otimes n')\\
      =&\;(1/d)\otimes (c\cdot n'),\\
    \end{align*}
    which is of the desired form. \\

    Now since elements of $Q\otimes_R N$ can
    be written as a finite sum of elements of the form $q\otimes n$ for
    some $q\in Q$ and $n\in N$, by induction on the number of sums, it
    suffices to show the sum of two elements $(1/d_1)\otimes n_1$ and
    $(1/d_2)\otimes n_2$ is of the desired form:
    \begin{align*}
      &\;(1/d_1)\otimes n_1 +(1/d_2)\otimes n_2\\
      =&\;(1/(d_1d_2))\otimes d_2n_1 +(1/(d_1d_2))\otimes d_1n_2
      &(\text{possible since}\; d_1,d_2\neq0)\\
      =&\;(1/(d_1d_2))\otimes(d_2n_1+d_1n_2),\\
    \end{align*}
    which is of the desired form since $d_1d_2\neq0$ because $R$ is an
    integral domain.
  \end{proof}

\it \textbf{Section 10.4 Q11:} Let $\{e_1,e_2\}$ be a basis of
  $V=\mathbb{R}^2$. Show that the element $e_1\otimes e_2+e_2\otimes e_1$
  in $V\otimes_\mathbb{R}V$ cannot be written as a simple tensor $v\otimes
  w$ for any $v,w\in\mathbb{R}^2$.

  \begin{proof}
    Consider the map $\varphi:V\times V\rightarrow\mathbb{R}^2$ defined by
    $\varphi\left(\left(\binom{r}{s},\binom{x}{y}\right)\right)
    =\binom{rx}{ry}$. It is routine to check that $\varphi$ is an
    $\mathbb{R}$-bilinear map. Thus by Corollary 12, $\varphi$ induces an
    $\mathbb{R}$-homomorphism
    $\Phi:V\otimes_\mathbb{R}V\rightarrow\mathbb{R}^2$ defined by
    $\Phi\left(\binom{r}{s}\otimes\binom{x}{y}\right) =\binom{rx}{ry}$.
    Thus if $\binom{r_1}{s_1}\otimes\binom{x_1}{y_1}
    =\binom{r_2}{s_2}\otimes\binom{x_2}{y_2} \in V\otimes V$, their image
    under $\Phi$ should be the same. In other words, we must have
    $r_1\binom{x_1}{y_1} =r_2\binom{x_2}{y_2}$. By a similar argument,
    swapping the roles of $s$ and $r$, we also get that if
    $\binom{r_1}{s_1}\otimes\binom{x_1}{y_1}
    =\binom{r_2}{s_2}\otimes\binom{x_2}{y_2} \in V\otimes V$ then
    $s_1\binom{x_1}{y_1} =s_2\binom{x_2}{y_2}$. We use these observations
    to check if two elements in $V\otimes V$ can be the same. \\

    In particular, if $\binom{r_1}{s_1}\otimes e_1 =\binom{r_2}{s_2}\otimes
    e_2$, then we must have $r_1\cdot e_1=r_2\cdot e_2$ and $s_1\cdot
    e_1=s_2\cdot e_2$. However, since $e_1$ and $e_2$ are linearly
    independent, we must have $r_1=r_2=s_1=s_2=0$. Thus $a\otimes e_1
    =b\otimes e_2$ if and only if $a=b=0$. Equivalently, $a\otimes e_1
    +b\otimes e_2=0$ has only trivial solutions $a=b=0\in V$. Thus, if
    \[r_{1,1}(e_1\otimes e_1) +r_{1,2}(e_1\otimes e_2) +r_{2,1}(e_2\otimes
      e_1) +r_{2,2}(e_2\otimes e_2)=0,\]
    for some $r_{1,1}=r_{1,2}=r_{2,1}=r_{2,2}\in\mathbb{R}$, then
    rearranging will give us
    \[(r_{1,1}e_1 +r_{2,1}e_2)\otimes e_1 +(r_{1,2}e_1 +r_{2,2}e_2)\otimes
      e_2=0\]
    Then from the above observation, we can only have trivial solutions
    \[r_{1,1}e_1 +r_{2,1}e_2 =r_{1,2}e_1 +r_{2,2}e_2 =0,\]
    which in turn only has trivial solutions
    $r_{1,1}=r_{1,2}=r_{2,1}=r_{2,2}=0$ since $e_1,e_2$ are linearly
    independent. \\

    Now assume $e_1\otimes e_2+e_2\otimes e_1 =v\otimes w$ for some $v,w\in
    V$. Then since $\{e_1,e_2\}$ is a basis of $\mathbb{R}^2$, we can write
    $v=r_1e_1+r_2e_2$ and $w=s_1e_1+s_2e_2$ for some
    $r_1,r_2,s_1,s_2\in\mathbb{R}$. Then
    \begin{align*}
      e_1\otimes e_2+e_2\otimes e_1 &=v\otimes w\\
      &=(r_1e_1+r_2e_2) \otimes(s_1e_1+s_2e_2)\\
      &=r_1s_1(e_1\otimes e_1) +r_1s_2(e_1\otimes e_2) +r_2s_1(e_2\otimes
        e_1) +r_2s_2(e_2\otimes e_2).\\
    \end{align*}
    Then from the previous argument, $v=w=0\in V$, thus $e_1\otimes
    e_2+e_2\otimes e_1=0$. But this would give a non-trivial solution for
    $a\otimes e_1+b\otimes e_2=0$, a contradiction.
  \end{proof}

\it \textbf{Section 10.4 Q12:} Let $V$ be a vector space over the field $F$
  and let $v,v'$ be nonzero elements of $V$. Prove that $v\otimes
  v'=v'\otimes v$ in $V\otimes_F V$ if and only if $v=av'$ for some $a\in
  F$.

  \begin{proof}
    The converse is trivial:
    \begin{align*}
      v\otimes v' &=av'\otimes v'\\
      &=a\cdot(v'\otimes v')\\
      &=v'\otimes av'\\
      &=v'\otimes v.\\
    \end{align*}

    For the forward direction. Let $\{e_i:i\in I\}$ be a
    basis of $V$. Assuming axiom of Choice, such a basis exists. Given
    $w\in V$, let $\alpha_i(w)\in F$ denote the coefficient of $e_i$ in the
    unique expression of $w$ as a linear sum of the basis elements. \\

    For each $i\in I$, consider the map $\varphi_i:V\times V\rightarrow V$
    defined by $\varphi_i((x,y))=\alpha_i(x)y$. It is routine to prove that
    $\varphi_i$ is an $F$-bilinear map. Thus by Corollary 12, $\varphi_i$
    induces an $F$-module homomorphism $\Phi_i:V\otimes_F V\rightarrow V$
    defined by $\Phi_i(x\otimes y)=\alpha_i(x)y$. Thus if $x_1\otimes
    y_1=x_2\otimes y_2\in V\otimes_F V$, then their images under $\Phi_i$
    for all $i\in I$ should be the same. In other words, we need
    $\alpha_i(x_1)y_1=\alpha_i(x_2)y_2$ for all $i\in I$. \\

    So assume $v\otimes v'=v'\otimes v \in V\otimes_F V$ where $v,v'\in V$
    are nonzero. Since $v'\neq0$, $\alpha_k(v')\neq0$ for some $k\in I$. So
    from the above argument, we have $\alpha_k(v)v'=\alpha_k(v')v$, which
    implies $v'$ and $v$ are linearly dependent since $\alpha_k(v)\neq0$.
    Then since $F$ is a field, $\alpha_k(v)$ has a multiplicative inverse.
    Rearranging, we get
    \[v=\alpha_k(v)\alpha_k(v')^{-1}v',\]
    where $\alpha_k(v)\alpha_k(v')^{-1} \in F$ as required.
  \end{proof}
\end{document}
